src/Distributions/Uniform/Equivalence.dfy
@@ -7,14 +7,13 @@ module Uniform.Equivalence {
   import Rand
   import Model
   import Monad
-  import Loops
 
   lemma SampleUnroll(n: nat, s: Rand.Bitstream)
     requires n > 0
     ensures Model.Sample(n)(s) == Monad.Bind(Model.Proposal(n), (x: nat) => if Model.Accept(n)(x) then Monad.Return(x) else Model.Sample(n))(s)
   {
-    Model.SampleTerminates(n);
+    //Model.SampleTerminates(n);
     reveal Model.Sample();
-    Loops.UntilUnroll(Model.Proposal(n), Model.Accept(n), s);
+    Monad.UntilUnroll(Model.Proposal(n), Model.Accept(n), s);
   }
 }
